foldl model

src/Std/Data/DHashMap/Internal/Defs.lean
@@ -448,8 +448,26 @@ def insertMany {ρ : Type w} [ForIn Id ρ ((a : α) × β a)] [BEq α] [Hashable
   return r
 
 /-- Internal implementation detail of the hash map -/
+@[inline] def foldl {δ : Type w} (f : δ → (a : α) → β a → δ) (init : δ)
+    (m : Raw₀ α β) : { d : δ // ∀ (P : δ → Prop),
+      (∀ {d' a b}, P d' → P (f d' a b)) → P init → P d } := Id.run do
+  let mut r : { d : δ // ∀ (P : δ → Prop),
+      (∀ {d' a b}, P d' → P (f d' a b)) → P init → P d } := ⟨init, fun _ _ => id⟩
+  for ⟨a, b⟩ in m.1 do
+    r := ⟨f r.1 a b, fun _ h hm => h (r.2 _ h hm)⟩
+  return r
+
+/-- Internal implementation detail of the hash map -/
+def interSmaller [BEq α] [Hashable α] (m₁ m₂ : Raw₀ α β) : Raw₀ α β :=
+  (m₂.foldl (fun sofar k _ => match m₁.getEntry? k with | some kv' => sofar.insert kv'.1 kv'.2 | none => sofar) emptyWithCapacity).1
+
+/-- Internal implementation detail of the hash map -/
 @[inline] def union [BEq α] [Hashable α] (m₁ m₂ : Raw₀ α β) : Raw₀ α β :=
   if m₁.1.size ≤ m₂.1.size then (m₂.insertManyIfNew m₁.1).1 else (m₁.insertMany m₂.1).1
+
+/-- Internal implementation detail of the hash map -/
+def inter [BEq α] [Hashable α] (m₁ m₂ : Raw₀ α β) : Raw₀ α β :=
+  if m₁.1.size ≤ m₂.1.size then m₁.filter fun k _ => m₂.contains k else interSmaller m₁ m₂
 
 section
 
