src/Std/Data/DHashMap/Basic.lean
@@ -319,6 +319,10 @@ This function always merges the smaller map into the larger map, so the expected
   inner := Raw₀.union ⟨m₁.1, m₁.2.size_buckets_pos⟩ ⟨m₂.1, m₂.2.size_buckets_pos⟩
   wf := Std.DHashMap.Raw.WF.union₀ m₁.2 m₂.2
 
+@[inline] def inter [BEq α] [Hashable α] (m₁ m₂ : DHashMap α β) : DHashMap α β where
+  inner := Raw₀.inter ⟨m₁.1, m₁.2.size_buckets_pos⟩ ⟨m₂.1, m₂.2.size_buckets_pos⟩
+  wf := sorry
+
 instance [BEq α] [Hashable α] : Union (DHashMap α β) := ⟨union⟩
 
 section Unverified
