src/Std/Data/DHashMap/Internal/WF.lean
@@ -1290,6 +1290,27 @@ theorem toListModel_union [BEq α] [Hashable α] [EquivBEq α] [LawfulHashable �
   rw [union_eq_unionₘ]
   exact toListModel_unionₘ h₁ h₂
 
+/-! # `foldl`-/
+theorem foldl_eq_foldlₘ {δ} (f : δ → (a : α) → β a → δ) (init : δ) (m : Raw₀ α β) :
+    foldl f init m = foldlₘ f init (m.1.toList) := by
+  simp [foldl,foldlₘ]
+  simp [ForIn.forIn]
+  rw [Raw.forIn_eq_forIn_toListModel]
+  rw [Raw.toList_eq_toListModel]
+  generalize (toListModel m.val.buckets) = l
+  simp only [forIn_pure_yield_eq_foldl, Id.run_pure]
+  suffices ∀ (t : { d : δ // ∀ (P : δ → Prop),
+      (∀ {d' : δ} {a : α} {b : β a}, P d' → P (f d' a b)) → P init → P d }),
+        (List.foldl (fun d' p => ⟨f d'.val p.1 p.2, fun P h₁ h₂ => h₁ (d'.2 _ h₁ h₂)⟩) t l).val =
+      foldlₘ f t.val l from this _
+  intro t
+  induction l generalizing t with
+  | nil => simp [foldlₘ]
+  | cons hd tl ih =>
+    simp only [List.foldl_cons, foldlₘ]
+    simp [foldlₘ] at ih
+    apply ih
+
 /-! # `Const.insertListₘ` -/
 
 theorem Const.toListModel_insertListₘ {β : Type v} [BEq α] [Hashable α] [EquivBEq α]
